prove most of the lemmas for well-formed command

language_formal/spark2014_semantics/propertyProof.v
@@ -1,9 +1,22 @@
 Require Export util.
 Require Export wellformed.
 
-(* TODO *)
-(* Right now the following is the assumption, which needs to be proved later. *)
+Inductive type_check_stack: symtb -> stack -> Prop :=
+    | TC_Empty: type_check_stack nil nil
+    | TC_Bool: forall tb s x m b,
+          type_check_stack tb s ->
+          type_check_stack ((x, (m, Tbool)) :: tb) ((x, (Value (Bool b))) :: s)
+    | TC_Int: forall tb s x m v,
+          type_check_stack tb s ->
+          type_check_stack ((x, (m, Tint)) :: tb) ((x, (Value (Int v))) :: s)
+    | TC_UndefBool: forall tb s x m,
+          type_check_stack tb s ->
+          type_check_stack ((x, (m, Tbool)) :: tb) ((x, Vundef) :: s)
+    | TC_UndefInt: forall tb s x m,
+          type_check_stack tb s ->
+          type_check_stack ((x, (m, Tint)) :: tb) ((x, Vundef) :: s).
 
+(*
 Inductive symbol_consistent: stack -> symtb -> Prop :=
     | SymCons: forall (s: stack) (tb: symtb), 
         ( forall x v, Some v = fetch x s -> 
@@ -12,17 +25,95 @@ Inductive symbol_consistent: stack -> symtb -> Prop :=
                           reside x s = true /\ 
                           (forall v, (Some v = fetch x s) -> stored_value_type (Value v) t)) -> 
         symbol_consistent s tb.
-
-(*
-Inductive return_value_type : return_val -> typ -> Prop :=
-    EVT_Int : forall n : Z, return_value_type (ValNormal (Int n)) Tint
-  | EVT_Bool : forall b : bool, return_value_type (ValNormal (Bool b)) Tbool
-
-Inductive stored_value_type : val -> typ -> Prop :=
-    SVT_Int : forall n : Z, stored_value_type (Value (Int n)) Tint
-  | SVT_Bool : forall b : bool, stored_value_type (Value (Bool b)) Tbool
-
 *)
+
+Lemma typed_value: forall tb s x v,
+    type_check_stack tb s ->
+    fetch x s = Some v ->
+    (exists t, stored_value_type (Value v) t /\ ( exists m, lookup x tb = Some (m, t))).
+Proof.
+    intros tb s x v h1 h2.
+    destruct v.
+  - exists Tint.
+    split.
+    + constructor.
+    + induction h1;
+       [inversion h2 | | | | ];
+       unfold fetch in h2;
+       unfold lookup;
+       destruct (beq_nat x x0);
+       [ inversion h2 | | exists m; auto | | inversion h2 | | inversion h2 | ];
+       fold fetch in h2;
+       fold lookup;
+       specialize (IHh1 h2);
+       assumption.
+  - exists Tbool.
+    split.
+    + constructor.
+    + induction h1;
+       [inversion h2 | | | | ];
+       unfold fetch in h2;
+       unfold lookup;
+       destruct (beq_nat x x0);
+       [ exists m; auto | | inversion h2 | | inversion h2 | | inversion h2 | ];
+       fold fetch in h2;
+       fold lookup;
+       specialize (IHh1 h2);
+       assumption.
+Qed.
+
+Ltac tv_l1 f1 f2 h1 h2 x x0 := 
+    unfold f1 in h1;
+    unfold f2;
+    destruct (beq_nat x x0);
+    [ auto |
+      fold f1 in h1;
+      fold f2;
+      specialize (h2 h1);
+      rm_exists; auto
+    ].
+
+Ltac tv_l2 f1 f2 h1 h2 x x0 tac :=
+    unfold f1 in h1;
+    unfold f2;
+    destruct (beq_nat x x0);
+    [ intros; 
+      inversion h1; subst;
+      inversion H; subst; 
+      tac |
+      fold f1 in h1;
+      fold f2;
+      specialize (h2 h1);
+      rm_exists; auto
+    ].
+
+Lemma typed_value': forall tb s x m t,
+    type_check_stack tb s ->
+    lookup x tb = Some (m, t) -> 
+    reside x s = true /\ 
+    (forall v, (Some v = fetch x s) -> stored_value_type (Value v) t).
+Proof.
+    intros tb s x m t h1 h2.
+    induction h1;
+    [inversion h2 | | | | ];
+    split;
+    [ | tv_l2 lookup fetch h2 IHh1 x x0 constructor |
+      | tv_l2 lookup fetch h2 IHh1 x x0 constructor |
+      | tv_l2 lookup fetch h2 IHh1 x x0 auto |
+      | tv_l2 lookup fetch h2 IHh1 x x0 auto
+    ];
+    tv_l1 lookup reside h2 IHh1 x x0.
+Qed.
+
+Inductive symbol_consistent1: stack -> symtb -> Prop :=
+    | SymCons: forall (s: stack) (tb: symtb), 
+        ( forall x v, Some v = fetch x s -> 
+                          (exists t, stored_value_type (Value v) t /\ ( exists m, lookup x tb = Some (m, t)))) -> 
+        (forall x m t, lookup x tb = Some (m, t) -> 
+                          reside x s = true /\ 
+                          (forall v, (Some v = fetch x s) -> stored_value_type (Value v) t)) -> 
+        symbol_consistent1 s tb.
+
 
 Ltac rm_contradict := 
     match goal with
@@ -39,9 +130,8 @@ Ltac rm_contradict2 :=
     | [h: return_value_type ValException ?t |- _] => destruct t; inversion h
     end.
 
-Lemma eval_type_reserve: 
-    forall (s: stack) (tb: symtb) e v t,
-    symbol_consistent s tb -> 
+Lemma eval_type_reserve: forall tb s e v t,
+    type_check_stack tb s -> 
     eval_expr s e v ->
     well_typed_expr tb e t ->
     return_value_type v t.
@@ -50,20 +140,19 @@ Proof.
     induction e;
     intros v t h1 h2 h3;
     inversion h3;
-    inversion h2; subst. 
+    inversion h2; subst.
   - (* Econst *)
     constructor.
   - constructor.  
   - (* Evar *)
-    inversion h1; subst.
-    symmetry in H3.
-    specialize (H0 i In t H3).
+    specialize (typed_value _ _ i v0 h1 ); intros hz1.
+    specialize (hz1 H8).
     rm_exists.
-    specialize (H2 _ H8).
+    rewrite H3 in H. inversion H; subst.
     apply value_type_consistent; assumption.
   - (* Ebinop *)
-    specialize (IHe1 v1 t0 h1 H14 H5).
-    specialize (IHe2 v2 t0 h1 H15 H6).
+    specialize (IHe1 _ _ h1 H14 H5).
+    specialize (IHe2 _ _ h1 H15 H6).
     destruct v1 as [v11 | v12]; try rm_contradict2.
     destruct v2 as [v21 | v22]; try rm_contradict2.
     destruct v11; destruct v21;
@@ -75,27 +164,68 @@ Proof.
   - (* Eunop *)
     unfold eval_unop; destruct op; simpl.
     constructor.
+(* another possible proof:
+    - - - - - - - - - - - - - - - - 
+    intros s tb e v t h1 h2.
+    generalize t.
+    induction h2; subst; 
+    intros t0 h3.
+  - (* Econst *)
+    inversion h3; subst;
+    constructor.
+  - (* Evar *)
+    inversion h3; subst.
+    inversion h1; subst.
+    specialize (H0 _ _ H).
+    rm_exists.
+    rewrite H2 in H4. 
+    inversion H4; subst.
+    apply value_type_consistent; assumption.
+  - (* Ebinop *)
+    inversion h3; subst.
+    specialize (IHh2_1 h1 _ H6).
+    specialize (IHh2_2 h1 _ H7).
+    destruct v1 as [v11 | v12]; try rm_contradict2.
+    destruct v2 as [v21 | v22]; try rm_contradict2.
+    destruct v11 as [v1i | v1b];
+    destruct v21 as [v2i | v2b];
+    inversion IHh2_1; subst.
+    ...
+*)
 Qed.
+
+Lemma exceptionVal_has_no_typ: forall tb s e t, 
+    type_check_stack tb s ->
+    eval_expr s e ValException -> 
+    well_typed_expr tb e t ->
+    False.
+Proof.
+    intros s tb e t h1 h2 h3.
+    specialize (eval_type_reserve _ _ _ _ _ h1 h2 h3).
+    intros h4.
+    destruct t; inversion h4.
+Qed.
+
 
 (* basic lemmas *)
 Ltac br_rm_rop v1 v2 op v1' v2' :=
     match goal with
     | [ |- exists v : value, eval_expr _ (Ebinop ?ast_id ?rop ?e1 ?e2) (ValNormal ?v)] =>
-            assert (exists b, ValNormal (Bool b) = eval_binop rop (ValNormal v1) (ValNormal v2))
+            assert (exists b, eval_binop rop (ValNormal v1) (ValNormal v2) = ValNormal (Bool b))
     end; [ simpl_binop; exists (op v1' v2'); auto | ].
 
 Ltac br_rm_aop v1 v2 v3 :=
     match goal with
     | [ |- exists v : value, eval_expr _ (Ebinop ?ast_id ?aop ?e1 ?e2) (ValNormal ?v)] =>
-            assert (exists n, ValNormal (Int n) = eval_binop aop (ValNormal v1) (ValNormal v2))
+            assert (exists n, eval_binop aop (ValNormal v1) (ValNormal v2) = ValNormal (Int n))
     end; [ simpl_binop; exists v3; auto | ].
 
 Ltac br_clearer v f :=
     exists v;
     rm_eval_expr; unfold f; auto.   
 
-Lemma binop_rule: forall s tb e1 v1 e2 v2 ast_id op t,
-    symbol_consistent s tb -> 
+Lemma binop_rule: forall tb s e1 v1 e2 v2 ast_id op t,
+    type_check_stack tb s -> 
     eval_expr s e1 (ValNormal v1) ->
     eval_expr s e2 (ValNormal v2) -> 
     well_typed_expr tb (Ebinop ast_id op e1 e2) t -> (* for example, disallow expression: 8 /\ 9 *)
@@ -103,8 +233,8 @@ Lemma binop_rule: forall s tb e1 v1 e2 v2 ast_id op t,
 Proof.    
     intros.
     inversion H2; subst.
-    specialize (eval_type_reserve s tb e1 (ValNormal v1) t0 H H0 H9); intros h1.
-    specialize (eval_type_reserve s tb e2 (ValNormal v2) t0 H H1 H10); intros h2.    
+    specialize (eval_type_reserve _ _ _ _ _ H H0 H9); intros h1.
+    specialize (eval_type_reserve _ _ _ _ _ H H1 H10); intros h2.    
     destruct v1 as [v11 | v12]; destruct v2 as [v21 | v22]; 
     inversion h1; subst; try rm_contradict. 
   - (* Ebinop Tint Tint *)
@@ -129,7 +259,7 @@ Qed.
 Ltac ru_rm_unop v1 v2 :=
     match goal with
     [ |- exists b : value, eval_expr _ (Eunop ?ast_id ?uop ?e) (ValNormal b)] => 
-            assert (exists b, ValNormal (Bool b) = eval_unop uop (ValNormal v1)) 
+            assert (exists b, eval_unop uop (ValNormal v1) = ValNormal (Bool b)) 
     end; 
     [simpl_unop; exists v2; auto | ].
 
@@ -137,24 +267,145 @@ Ltac ur_clearer v :=
     exists v;
     eapply eval_Eunop; eassumption.   
 
-Lemma unop_rule: forall s tb e v ast_id op t,
-    symbol_consistent s tb -> 
+
+Lemma unop_rule: forall tb s e v ast_id op t,
+    type_check_stack tb s -> 
     eval_expr s e (ValNormal v) ->
     well_typed_expr tb (Eunop ast_id op e) t -> 
     (exists bv : value, eval_expr s (Eunop ast_id op e) (ValNormal bv)).
 Proof.
     intros.
     inversion H1; subst.
-    specialize (eval_type_reserve s tb e (ValNormal v) Tbool H H0 H6); 
+    specialize (eval_type_reserve _ _ _ _ _ H H0 H6); 
     intros h1.
     destruct v; try rm_contradict.
     destruct op.
     ru_rm_unop (Bool b) (negb b).
     rm_exists.  
     ur_clearer (Bool x).
-Qed. 
+Qed.
 
-Theorem well_formed_expr: forall tb s e t,
+Lemma well_formed_expr: forall tb s e t,
+    type_check_stack tb s -> 
+    well_defined_expr s e ->
+    well_typed_expr tb e t ->
+    exists v, eval_expr s e v /\ return_value_type v t.
+Proof.
+    intros tb s e t h1 h2.
+    generalize t. 
+    induction h2; 
+    intros t0 h3.
+    (* 1. Econst *)
+  - exists (ValNormal (Int n)).
+    split.
+    + constructor. 
+       unfold eval_constant; simpl; auto.
+    + inversion h3; subst.
+       constructor.
+  - exists (ValNormal (Bool b)).
+    split.
+    + constructor. 
+       unfold eval_constant; simpl; auto.
+    + inversion h3; subst.
+       constructor.
+    (* 2. Evar *)
+  - exists (ValNormal v).
+    assert (HZ1: eval_expr s (Evar ast_id x) (ValNormal v)). (* this one is used to prove "return_value_type _ _" *)
+    constructor; assumption.
+    split.
+    + assumption.
+    + apply eval_type_reserve with (s := s) (tb := tb) (e := (Evar ast_id x));
+       assumption.
+    (* 3. Ebinop *)
+  - assert (HZ2: exists v, eval_expr s (Ebinop ast_id op e1 e2) v).
+    inversion h3; subst. 
+    specialize (IHh2_1 h1 _ H5).
+    specialize (IHh2_2 h1 _ H6).
+    rm_exists.
+
+    destruct x; destruct x0.
+    + specialize (binop_rule _ _ _ _ _ _ _ _ _ h1 H1 H0 h3).
+       intros h4; rm_exists. 
+       exists (ValNormal x); assumption.
+    + specialize (exceptionVal_has_no_typ _ _ _ _ h1 H1 H5); intuition.
+    + specialize (exceptionVal_has_no_typ _ _ _ _ h1 H0 H6); intuition.
+    + specialize (exceptionVal_has_no_typ _ _ _ _ h1 H0 H6); intuition.
+    
+    + rm_exists. 
+       exists x. 
+       split; try assumption.
+       apply eval_type_reserve with (s := s) (tb := tb) (e := (Ebinop ast_id op e1 e2));
+       assumption.
+    (* 4. Eunop *)
+  - assert(HZ3: exists v, eval_expr s (Eunop ast_id op e) v ).
+    inversion h3; subst.
+    specialize (IHh2 h1 _ H3).
+    rm_exists.
+    specialize (eval_type_reserve _ _ _ _ _ h1 H0 H3).
+    intros h5.
+    destruct x; try rm_contradict.
+    destruct v; try rm_contradict.
+    set (y :=  (eval_unop op (ValNormal (Bool b)))).
+    exists y. 
+    econstructor. 
+    apply H0. intuition.
+    
+    rm_exists.
+    exists (x).
+    split; try assumption.
+    apply eval_type_reserve with (s := s) (tb := tb) (e := (Eunop ast_id op e));
+    assumption.
+Qed.
+
+
+Lemma well_formed_expr_lm: forall tb s e t,
+    type_check_stack tb s -> 
+    well_defined_expr s e ->
+    well_typed_expr tb e t ->
+    exists v, eval_expr s e v.
+Proof.
+    intros tb s e t h1 h2.
+    generalize t. 
+    induction h2; 
+    intros t0 h3.
+    (* 1. Econst *)
+  - exists (ValNormal (Int n)).
+    constructor. unfold eval_constant; simpl; auto.
+  - exists (ValNormal (Bool b)).
+    constructor. unfold eval_constant; simpl; auto.
+    (* 2. Evar *)
+  - exists (ValNormal v).
+    constructor; assumption.
+    (* 3. Ebinop *)
+  - inversion h3; subst. 
+    specialize (IHh2_1 h1 _ H5).
+    specialize (IHh2_2 h1 _ H6).
+    rm_exists.
+
+    destruct x; destruct x0.
+    + specialize (binop_rule _ _ _ _ _ _ _ _ _ h1 H0 H h3).
+       intros h4; rm_exists. 
+       exists (ValNormal x); assumption.
+    + specialize (exceptionVal_has_no_typ _ _ _ _ h1 H0 H5); intuition.
+    + specialize (exceptionVal_has_no_typ _ _ _ _ h1 H H6); intuition.
+    + specialize (exceptionVal_has_no_typ _ _ _ _ h1 H H6); intuition.
+
+    (* 4. Eunop *)
+  - inversion h3; subst.
+    specialize (IHh2 h1 _ H3).
+    rm_exists.
+    specialize (eval_type_reserve _ _ _ _ _ h1 H H3).
+    intros h5.
+    destruct x; try rm_contradict.
+    destruct v; try rm_contradict.
+    set (y :=  (eval_unop op (ValNormal (Bool b)))).
+    exists y. 
+    econstructor. 
+    apply H. intuition.
+Qed.
+
+(*
+Lemma well_formed_expr_lm: forall tb s e t,
     well_typed_expr tb e t ->
     well_defined_expr s e ->
     symbol_consistent s tb -> 
@@ -196,25 +447,21 @@ Proof.
 
     * (* 3.2 ValInt, ValBool *)
       inversion H2. inversion H3.
-      specialize (eval_type_reserve s tb e1 (ValNormal (Int x)) t0 H1 H4 H8); intros.
-      specialize (eval_type_reserve s tb e2 (ValNormal (Bool x0)) t0 H1 H6 H9); intros.
-      inversion H7; subst. inversion H12.
+      specialize (eval_type_reserve _ _ _ _ _ H1 H4 H8); intros.
+      specialize (eval_type_reserve _ _ _ _ _ H1 H6 H9); intros.
+      inversion H7; subst. 
+      inversion H12.
     * (* 3.3 ValBool, ValInt *)
       inversion H2. inversion H3.
-      specialize (eval_type_reserve s tb e1 (ValNormal (Bool x)) t0 H1 H4 H8); intros.
-      specialize (eval_type_reserve s tb e2 (ValNormal (Int x0)) t0 H1 H6 H9); intros.
+      specialize (eval_type_reserve _ _ _ _ _ H1 H4 H8); intros.
+      specialize (eval_type_reserve _ _ _ _ _ H1 H6 H9); intros.
       inversion H7; subst. inversion H12.
     * (* 3.4 ValBool, ValBool *)
       inversion H2. inversion H3.
-
-      specialize (binop_rule s tb e1 (Bool x) e2 (Bool x0) a b t H1 H4 H6 H).
+      specialize (binop_rule _ _ _ _ _ _ _ _ _ H1 H4 H6 H).
       intros h2. inversion h2. destruct x1 as [x2 | x3]. 
       left; exists x2; assumption.
       right; exists x3; assumption.
-(*      
-      specialize (binop_ind' s tb a b e1 e2 x x0 t H4 H6 H H1). 
-      intros. right; apply H7.
-*)
   - (* 4. Eunop *)
     inversion H; subst. 
     inversion H0; subst.
@@ -230,31 +477,523 @@ Proof.
        right; exists x3; assumption.
 Qed.
 
-(* = = = = = = = = = = = = = = =  *)
-(* = = = = = = = = = = = = = = =  *)
+Theorem well_formed_expr: forall tb s e t,
+    well_typed_expr tb e t ->
+    well_defined_expr s e ->
+    symbol_consistent s tb -> 
+    exists v, eval_expr s e v /\ return_value_type v t.
+Proof.
+    intros tb s e t h1 h2 h3.
+    specialize (well_formed_expr_lm _ _ _ _ h1 h2 h3).
+    intros h.
+    rm_or_hyp; rm_exists.
+  - exists (ValNormal (Int x)).
+    split.
+    + assumption.
+    + apply eval_type_reserve with (s := s) (tb := tb) (e := e);
+       assumption.
+  - exists (ValNormal (Bool x)).
+    split.
+    + assumption.
+    + apply eval_type_reserve with (s := s) (tb := tb) (e := e);
+       assumption.
+Qed.
+*)
 
-Axiom valid_update: forall s tb ast_id x e v,
-    symbol_consistent s tb ->
-    well_typed_stmt tb (Sassign ast_id x e) ->
-    exists s', update s x (Value v) = Some s'.
+(* = = = = = = = = = = = = = = =  *)
+(* = = = = = = = = = = = = = = =  *)
 
 (* -> *)
-Axiom equal_wd_expr_expr2_R: forall s istate e,  
+Lemma equal_wd_expr_expr2_R: forall s istate e,  
     initializationMap s istate ->
     well_defined_expr s e -> 
-    well_defined_expr2 istate e.
+    well_defined_expr2 istate e. (* !!! *)
+Proof.
+    intros s istate e h1 h2.
+    induction h2; try constructor; try intuition. 
+  - apply initializationMap_consistent1 with (s:=s) (v:=v);
+    assumption.
+Qed.
 
 (* <- *)    
-Axiom equal_wd_expr_expr2_L: forall s istate e,
+Lemma equal_wd_expr_expr2_L: forall s istate e,
     initializationMap s istate ->
     well_defined_expr2 istate e -> 
-    well_defined_expr s e.
+    well_defined_expr s e. (* !!! *)
+Proof.
+    intros s istate e h1 h2.
+    induction h2; try constructor; try intuition.
+  - specialize (initializationMap_consistent2 _ _ _ h1 H); intros h3.
+    rm_exists.
+    apply WD_Evar with (v:=x0).
+    auto. 
+Qed.
 
-Axiom symbol_consistent_reserve: forall s tb k c s',
-     symbol_consistent s tb -> 
-     f_eval_stmt k s c = SNormal s' -> 
-     symbol_consistent s' tb.
+Lemma valid_update: forall tb s ast_id x e v,
+    type_check_stack tb s ->
+    well_typed_stmt tb (Sassign ast_id x e) ->
+    exists s', update s x (Value v) = Some s'.  (* !!! *)
+Proof.
+    intros tb s ast_id x e v h1 h2.
+    inversion h2; subst.
+    specialize (typed_value' _ _ _ Out t h1 H2); intros hz1.
+    rm_exists.
+    clear h1 h2 H0 H2 H4.
+    functional induction (reside x s).
+    + unfold update; rewrite e1.
+       exists ((y, Value v) :: s'); auto.
+    + specialize (IHb H).
+       rm_exists.
+       unfold update.
+       rewrite e1.
+       fold update.
+       rewrite H0. 
+       exists ((y, v0) :: x0); auto.
+    + inversion H.
+Qed.
 
+Lemma type_reserve: forall s x v s' tb m t ,
+    update s x (Value v) = Some s' ->    
+    type_check_stack tb s -> 
+    lookup x tb = Some (m, t)-> 
+    return_value_type (ValNormal v) t ->
+    type_check_stack tb s'. (* !!! *)
+Proof.
+    intros s x v.
+    remember (Value v) as v'0.
+    functional induction (update s x v'0);
+    intros s'0 tb m t h1 h2 h3 h4.
+  - inversion h1; clear h1; subst.
+    destruct tb. 
+    + inversion h3.
+    + destruct p.
+       inversion h2; subst;
+       unfold lookup in h3; rewrite e0 in h3; fold lookup;
+       inversion h3; clear h3; subst;
+       destruct v;
+       [ rm_contradict | | | rm_contradict | rm_contradict | | | rm_contradict ];
+       constructor; assumption.
+  - inversion h1; subst.
+    destruct tb.
+    + inversion h3.
+    + assert (hz1: Value v = Value v); auto.
+       destruct p; 
+       inversion h2; subst;
+       constructor;
+       unfold lookup in h3; rewrite e0 in h3; fold lookup in h3;
+       specialize (IHo hz1 _ _ _ _ e1 H0 h3 h4);
+       assumption.
+  - inversion h1.
+  - inversion h1.
+Qed.
+
+Lemma type_reserve_assign: forall tb s ast_id x e v s',
+    type_check_stack tb s -> 
+    well_typed_stmt tb (Sassign ast_id x e) -> 
+    eval_expr s e (ValNormal v) ->
+    update s x (Value v) = Some s' ->
+    type_check_stack tb s'. (* !!! *)
+Proof.
+    intros tb s ast_id x e v s' h1 h2 h3 h4.
+    inversion h2; subst.
+    specialize (eval_type_reserve _ _ _ _ _ h1 h3 H4); intros hz1.
+    specialize (type_reserve _ _ _ _ _ _ _ h4 h1 H2 hz1); intros hz2.
+    assumption.
+Qed.
+
+Lemma symbol_consistent_reserve: forall tb s c s',
+    type_check_stack tb s -> 
+    well_typed_stmt tb c ->
+    eval_stmt s c s' ->  (* the assignment does not check the type consistency *)
+    type_check_stack tb s'. (* !!! *)
+Proof.
+    intros tb s c s' h1 h2 h3.
+    induction h3.
+  - (* Sassign *)
+    specialize (type_reserve_assign _ _ _ _ _ _ _ h1 h2 H H0); intros hz1.
+    assumption.
+  - inversion h2; subst.
+    apply IHh3_2.
+    apply IHh3_1;
+    assumption.
+    assumption.
+  - inversion h2; subst.
+    apply IHh3;
+    assumption.
+  - inversion h2; subst.
+    assumption.
+  - inversion h2; subst.
+    apply IHh3_2.
+    apply IHh3_1;
+    assumption.
+    assumption.
+  - inversion h2; subst.
+    assumption.
+Qed.
+
+
+Lemma imap_exists: forall s, 
+    exists istate, initializationMap s istate.
+Proof.
+    intros s.
+    induction s.
+    exists nil; constructor.
+    rm_exists.
+    destruct a.
+    destruct v.
+  - exists ((i, Init) :: x); constructor. 
+    intuition. inversion H0.
+    assumption.
+  - exists ((i, Uninit) :: x); constructor.
+    auto.
+    assumption.
+Qed.
+
+(****************************************************)
+(****************************************************)
+(*
+Axiom istate_preserve: forall istate e c istate',
+    well_defined_expr2 istate e ->
+    well_defined_stmt2 istate c istate' ->
+    well_defined_expr2 istate' e.
+*)
+
+Lemma initializationMap_expr: forall istate1 e istate2,
+     well_defined_expr2 istate1 e ->   
+     (forall x, fetch2 x istate1 = Some Init -> fetch2 x istate2 = Some Init) ->
+     well_defined_expr2 istate2 e.
+Proof.
+    intros istate1 e istate2 h1.
+    generalize istate2. 
+    clear istate2.
+    induction e;
+    intros istate2 h2.
+  - destruct c; constructor.
+  - inversion h1; subst.
+    specialize (h2 _ H1).
+    constructor. assumption.
+  - inversion h1; subst.
+    constructor.
+    + specialize (IHe1 H2 _ h2).
+       assumption.
+    + specialize (IHe2 H5 _ h2).
+       assumption.
+  - inversion h1; subst.
+    constructor.
+    specialize (IHe H1 _ h2).
+    assumption.
+Qed.
+
+(* this modified version is used to prove lemma: ''initializationMap_stmt'' *)
+Lemma initializationMap_expr1: forall istate1 e istate2,
+     well_defined_expr2 istate1 e ->   
+     (forall x, (fetch2 x istate1 = Some Init -> fetch2 x istate2 = Some Init) /\
+                   (fetch2 x istate1 = Some Uninit -> exists m, fetch2 x istate2 = Some m)) ->
+     well_defined_expr2 istate2 e.
+Proof.
+    intros.
+    distr_qualifier.
+    specialize (initializationMap_expr _ _ _ H H0); intros hz1.
+    assumption.
+Qed.
+
+Lemma fetch2_transitive: forall istate1 istate2 istate3,
+    (forall x : idnum,
+      (fetch2 x istate1 = Some Init -> fetch2 x istate2 = Some Init) /\
+      (fetch2 x istate1 = Some Uninit ->
+       exists m : init_mode, fetch2 x istate2 = Some m)) ->       
+    (forall x : idnum,
+      (fetch2 x istate2 = Some Init -> fetch2 x istate3 = Some Init) /\
+      (fetch2 x istate2 = Some Uninit ->
+       exists m : init_mode, fetch2 x istate3 = Some m)) ->
+    (forall x : idnum,
+      (fetch2 x istate1 = Some Init -> fetch2 x istate3 = Some Init) /\
+      (fetch2 x istate1 = Some Uninit ->
+       exists m : init_mode, fetch2 x istate3 = Some m)).
+Proof.
+    intros istate1 istate2 istate3 h1 h2.
+    intros x.
+    repeat distr_qualifier.
+    split; intros hz1.
+  - apply H0.
+    apply H2; assumption.
+  - specialize (H3 _ hz1).
+    rm_exists.
+    destruct x0 as [x1 | x2].
+    + specialize (H0 _ H).
+       exists Init; assumption.
+    + specialize (H1 _ H).
+       assumption.
+Qed.
+
+(* 'c' is put before 'istate1', because when we do induction on 'c', keep 'istate1' universal *)
+Lemma wd_fetch2_sync: forall c istate1 istate1' istate2 istate2',
+    well_defined_stmt2 istate1 c istate1' ->
+    well_defined_stmt2 istate2 c istate2' ->
+    (forall x, (fetch2 x istate1 = Some Init -> fetch2 x istate2 = Some Init) /\
+                  (fetch2 x istate1 = Some Uninit -> exists m', fetch2 x istate2 = Some m')) ->
+    (forall x, (fetch2 x istate1' = Some Init -> fetch2 x istate2' = Some Init) /\
+                  (fetch2 x istate1' = Some Uninit -> exists m', fetch2 x istate2' = Some m')).
+Proof.
+    induction c;
+    intros istate1 istate1' istate2 istate2' h1 h2 h3.
+  - distr_qualifier.
+    inversion h1; subst.
+    inversion h2; subst.
+    intros x.
+    split; intros hz1.
+    + specialize (update2_in1 _ _ _ _ _ _ H7 hz1); intros hz2.
+       inversion hz2 as [hz3 | hz4].
+       * inversion hz3; subst.
+         specialize (update2_fetch2_new _ _ _ _  H9). 
+         auto.
+       * rm_exists.
+         specialize (H0 _ H2).
+         specialize (update2_fetch2_old _ _ _ _ _ H9 H); intros hz3.
+         rewrite H0 in hz3.
+         assumption.
+    + specialize (update2_in1 _ _ _ _ _ _ H7 hz1); intros hz2.
+       inversion hz2 as [hz3 | hz4].
+       * inversion hz3.
+          inversion H2.
+       * rm_exists.
+         specialize (H1 _ H2).
+         specialize (update2_fetch2_old _ _ _ _ _ H9 H); intros hz3.
+         rewrite hz3.
+         assumption.
+  - distr_qualifier.
+    inversion h1; subst.
+    inversion h2; subst.
+    intros x.
+    split; intros hz1.
+    specialize (H0 _ hz1); assumption.
+    specialize (H1 _ hz1); assumption.
+  - distr_qualifier.
+    inversion h1; subst.
+    inversion h2; subst.
+    intros x.
+    split; intros hz1.
+    specialize (H0 _ hz1); assumption.
+    specialize (H1 _ hz1); assumption.
+  - inversion h1; subst.
+    inversion h2; subst.
+    intros x.
+    split; intros hz1;
+    specialize (IHc1 _ _ _ _ H4 H6 h3);
+    specialize (IHc2 _ _ _ _ H5 H7 IHc1);
+    repeat distr_qualifier.
+    + apply H2. assumption.
+    + apply H3. assumption.
+Qed.
+
+Lemma initializationMap_stmt: forall istate1 c istate1' istate2,
+     well_defined_stmt2 istate1 c istate1' ->   
+     (forall x, (fetch2 x istate1 = Some Init -> fetch2 x istate2 = Some Init) /\
+                   (fetch2 x istate1 = Some Uninit -> exists m, fetch2 x istate2 = Some m)) ->
+     exists istate2', well_defined_stmt2 istate2 c istate2'.
+Proof.
+    intros istate1 c istate1' istate2 h1.
+    generalize istate2. clear istate2.
+    induction h1;
+    intros istate2 h2.
+  - specialize (initializationMap_expr1 _ _ _ H h2); intros hz1.
+    assert (hz2: exists istate, update2 istate2 x Init = Some istate).
+    + distr_qualifier.
+       specialize (update2_fetch2 _ _ _ _ H0); intros hz2.
+       rm_exists. 
+       destruct x0.
+       * specialize (H2 _ H1).
+         specialize (fetch2_update2 _ _ _ Init H2); intros hz3.
+         assumption.
+       * specialize (H3 _ H1).
+         inversion H3.
+         specialize (fetch2_update2 _ _ _ Init H4); intros hz4.
+         assumption.
+    + rm_exists.
+       exists x0.
+       constructor; assumption.
+  - specialize (IHh1_1 _ h2).
+    rm_exists.
+    assert (hz2: forall y : idnum, (fetch2 y s' = Some Init -> fetch2 y x = Some Init) /\ 
+                                                 (fetch2 y s' = Some Uninit -> exists m', fetch2 y x = Some m')).
+    + specialize (wd_fetch2_sync _ _ _ _ _ h1_1 H h2); intros hz1.
+       assumption.
+    + specialize (IHh1_2 x hz2).
+       rm_exists.
+       exists x0.
+       apply WD_Sseq2 with (s' := x);
+       assumption.
+  - exists istate2.
+    specialize (IHh1 _ h2).
+    rm_exists.
+    apply WD_Sifthen2 with (s' := x).    
+    + distr_qualifier.
+       specialize (initializationMap_expr _ _ _ H H2); intros hz1.
+       assumption.
+    + assumption.
+  - exists istate2.
+    specialize (IHh1 _ h2).
+    rm_exists.
+    apply WD_Swhile2 with (s' := x).
+    + distr_qualifier.
+       specialize (initializationMap_expr _ _ _ H H2); intros hz1.
+       assumption.
+    + assumption.
+Qed.
+
+
+Lemma initializationMap_inc: forall istate c istate',
+     well_defined_stmt2 istate c istate' ->   
+     (forall x, (fetch2 x istate = Some Init -> fetch2 x istate' = Some Init) /\
+                   (fetch2 x istate = Some Uninit -> exists m, fetch2 x istate' = Some m)).
+Proof.
+    intros istate c istate' h1.
+    induction h1; 
+    intros x0.
+  - split; intros;
+    remember (beq_nat x0 x) as eq;
+    symmetry in Heqeq;
+    destruct eq as [eq1 | eq2].
+       * apply beq_nat_true in Heqeq.
+         subst.
+         specialize (update2_fetch2_new _ _ _ _ H0); intros hz1.
+         assumption.
+       * apply beq_nat_false in Heqeq.
+         specialize (update2_fetch2_old _ _ _ _ _ H0 Heqeq); intros hz1.
+         rewrite hz1.
+         assumption.
+       * apply beq_nat_true in Heqeq.
+         subst.
+         specialize (update2_fetch2_new _ _ _ _ H0); intros hz1.
+         exists Init; assumption.
+       * apply beq_nat_false in Heqeq.
+         specialize (update2_fetch2_old _ _ _ _ _ H0 Heqeq); intros hz1.
+         rewrite hz1.
+         exists Uninit; assumption.         
+  - repeat distr_qualifier.
+    split; intros hz1.
+    + apply H0.
+       apply H2.
+       assumption.
+    + specialize (H3 _ hz1).
+       rm_exists.
+       destruct x.
+       specialize (H0 _ H).
+       exists Init; assumption.
+       specialize (H1 _ H).
+       assumption.
+  - split.
+    + auto.
+    + intros.
+       exists Uninit.
+       assumption.
+  - split.
+    + auto.
+    + intros.
+       exists Uninit.
+       assumption.
+Qed.
+
+Lemma eval_stmt_greater: forall s c s' istate istate' istate1,
+     eval_stmt s c s' -> 
+     initializationMap s istate ->
+     well_defined_stmt2 istate c istate' -> 
+     initializationMap s' istate1 -> 
+     (forall x, (fetch2 x istate' = Some Init -> fetch2 x istate1 = Some Init) /\
+                   (fetch2 x istate' = Some Uninit -> exists m, fetch2 x istate1 = Some m)).
+Proof.
+    intros s c s' istate istate' istate1 h1.
+    generalize istate istate' istate1.
+    clear istate istate' istate1.
+    induction h1;
+    intros istate istate' istate1 h2 h3 h4.
+  - (* 1. Sassign *)
+    inversion h3; subst.
+    specialize (update_consis _ _ _ _ _ _ _ h2 H0 H7 h4); intros hz1.
+    subst.
+    intros. 
+    split; intros.
+    + assumption.
+    + exists Uninit.
+       assumption.
+  - (* 2. Sseq *)
+    inversion h3; subst.
+    specialize (imap_exists s1); intros hz1.
+    rm_exists.
+    specialize (IHh1_1 _ _ _ h2 H4 H).
+    assert (hz2: exists istate, well_defined_stmt2 x c2 istate).
+    specialize (initializationMap_stmt _ _ _ _ H5 IHh1_1); intros hz2.
+    assumption.
+    rm_exists.
+    specialize (IHh1_2 _ _ _ H H0 h4).
+    specialize (wd_fetch2_sync _ _ _ _ _ H5 H0 IHh1_1); intros hz3.
+    specialize (fetch2_transitive _ _ _ hz3 IHh1_2); intros hz4.
+    assumption.
+  - (* 3. Sifthen_true *)
+    inversion h3; subst.
+    specialize (IHh1 _ _ _ h2 H6 h4).
+    specialize (initializationMap_inc _ _ _ H6); intros hz1.
+    specialize (fetch2_transitive _ _ _ hz1 IHh1); intros hz2.
+    assumption.
+  - (* 4. Sifthen_false *)
+    inversion h3; subst.
+    specialize (initializationMap_unique _ _ _ h4 h2); intros hz3.
+    subst.
+    intros x.
+    split; intros hz.
+    + assumption.
+    + exists Uninit; assumption.
+  - (* 5. Swhile_true *)
+    inversion h3; subst.
+    specialize (imap_exists s1); intros hz1.
+    rm_exists.
+    specialize (IHh1_1 _ _ _ h2 H6 H0).
+    specialize (initializationMap_inc _ _ _ H6); intros hz2.
+    assert (hz2': exists istate, well_defined_stmt2 x (Swhile ast_id b c) istate).
+    exists x.
+    assert (hz3: exists istate, well_defined_stmt2 x c istate).
+    specialize (initializationMap_stmt _ _ _ _ H6 hz2); intros hz3.
+    inversion hz3.
+    specialize (initializationMap_stmt _ _ _ _ H1 IHh1_1); intros hz4.    
+    assumption.
+    inversion hz3.
+    apply WD_Swhile2 with (s' := x0). 
+    + specialize (fetch2_transitive _ _ _ hz2 IHh1_1); intros hz5.
+       specialize (initializationMap_expr1 _ _ _ H5 hz5); intros hz6.
+       assumption.
+    + assumption.
+    + inversion hz2'.
+       inversion H1; subst.
+       specialize (IHh1_2 _ _ _ H0 H1 h4).
+       specialize (fetch2_transitive _ _ _ IHh1_1 IHh1_2); intros hz3.
+       specialize (fetch2_transitive _ _ _ hz2 hz3); intros hz4.
+       assumption.
+  - (* 6. Swhile_false *)
+    inversion h3; subst.
+    specialize (initializationMap_unique _ _ _ h4 h2); intros hz3.
+    subst.
+    intros x.
+    split; intros hz.
+    + assumption.
+    + exists Uninit; assumption.
+Qed.
+
+Lemma initializationMap_consistent: forall s istate c1 s' istate' c2 istate'' istate1,
+     initializationMap s istate ->
+     eval_stmt s c1 s' -> 
+     well_defined_stmt2 istate c1 istate' -> 
+     well_defined_stmt2 istate' c2 istate'' ->      
+     initializationMap s' istate1 ->
+     exists istate2, well_defined_stmt2 istate1 c2 istate2.
+Proof.
+    intros s istate c1 s' istate' c2 istate'' istate1 h1 h2 h3 h4 h5.
+    specialize (eval_stmt_greater _ _ _ _ _ _ h2 h1 h3 h5); intros hz1.
+    specialize (initializationMap_stmt _ _ _ _ h4 hz1); intros hz2.
+    assumption.
+Qed.
+
+
+(*
 Axiom imap_exists: forall s, exists istate, 
     initializationMap s istate.
 
@@ -271,6 +1010,14 @@ Axiom type_consistent: forall s tb b v,
     well_typed_expr tb b Tbool ->
     ~eval_expr s b (ValNormal (Int v)).  
 
+Axiom while_well_form : forall s tb b k c s' ast_id,
+    symbol_consistent s tb ->
+    well_defined_expr s b -> 
+    well_typed_expr tb b Tbool ->
+    f_eval_stmt k s c = SNormal s' ->
+        (exists s'0 : stack, f_eval_stmt k s' (Swhile ast_id b c) = SNormal s'0) \/
+        f_eval_stmt k s' (Swhile ast_id b c) = SUnterminated.
+
 Axiom initializationMap_Expr: forall (s: stack) istate e k c s' istate',
     initializationMap s istate ->
     well_defined_expr2 istate e ->
@@ -284,105 +1031,125 @@ Axiom initializationMap_Stmt: forall (s: stack) istate k c s' istate' istate1,
     well_defined_stmt2 istate c istate' ->
     initializationMap s' istate1 ->
     exists istate2, well_defined_stmt2 istate1 c istate2.
+*)
 
+
+Ltac unfold_f_eval_stmt :=
+    match goal with
+    | [ |- context[f_eval_stmt ?k ?s _]] => unfold f_eval_stmt; simpl
+    end.
+
+(*
+Ltac invert_well_form_hyp :=
+    match goal with 
+    | [h: well_defined_stmt2 _ (Sassign _ ?x ?e) _ |- _] => inversion h; subst
+    | [h: well_typed_stmt _ (Sassign _ ?x ?e) |- _] => inversion h; subst
+    | [h: well_defined_stmt2 _ (Sifthen _ ?b ?c) _ |- _] => inversion h; subst
+    | [h: well_typed_stmt _ (Sifthen _ ?b ?c) |- _] => inversion h; subst
+    | [h: well_defined_stmt2 _ (Swhile _ ?b ?c) _ |- _] => inversion h; subst
+    | [h: well_typed_stmt _ (Swhile _ ?b ?c) |- _] => inversion h; subst
+    end.
+*)
 
 (* Lemmas to prove... *)
-Lemma well_formed_cmd: forall k s tb c istate istate', 
-    symbol_consistent s tb ->
+Lemma well_formed_cmd: forall tb c s istate istate' k, 
+    well_typed_stmt tb c -> (* we want to do induction on 'c', but keep the variables 's', 'istate' ... universal *)
+    type_check_stack tb s ->
     initializationMap s istate ->
-    well_typed_stmt tb c ->
     well_defined_stmt2 istate c istate' ->
     (exists s', f_eval_stmt k s c = (SNormal s')) \/ f_eval_stmt k s c = SUnterminated.
 Proof.
-    intros k s tb c. 
-    functional induction (f_eval_stmt k s c);
-    intros istate istate' h1 h2 h3 h4;
-    try intuition.
-  - left.
-    exists s1. auto.
-  - left. 
-    (**)specialize (valid_update s tb ast_id x e0 v h1 h3). intros h5.
-    inversion h5; subst.
-    rewrite e3 in H. inversion H.
-  - inversion h4; subst.
-    inversion h3; subst.
-    (**)specialize (equal_wd_expr_expr2_L s istate e0 h2 H4). intros h6.
-    specialize (well_formed_expr tb s e0 t H6 h6 h1). intros.
-    inversion H; inversion H0.
-    + specialize (f_eval_expr_complete s e0 (ValNormal (Int x0)) H1). intros h7.
-       rewrite e2 in h7. inversion h7.
-    + specialize (f_eval_expr_complete s e0 (ValNormal (Bool x0)) H1). intros h7.
-       rewrite e2 in h7. inversion h7.
-  - (* Cseq *) 
-    inversion h3; subst.
+    intros tb. 
+    (* in the later proof during the induction on 'c', we have to keep the variables 's', 'istate', 'istate'', 'k' 
+       universal, that's why in the definition of lemma, we put 'well_typed_stmt' at the beginning  *)
+    induction c;
+    intros s istate istate' k h1 h2 h3 h4.
+  - (* 1. Sassign *)
+    inversion h1; subst.
     inversion h4; subst.
-    specialize (IHs0 istate s' h1 h2 H2 H6).
-    (**)specialize (symbol_consistent_reserve s tb k' c1 s1 h1 e1). intros h8.
-    specialize (imap_exists s1). intros h9. inversion h9; clear h9.
-
-    (**)specialize (initializationMap_consistent s istate k' s c1 s1 s' c2 istate' x h2 e1 H6 H7 H). intros h9.
-    inversion h9.    
-    specialize (IHs1 x x0 h8 H H4 H0). assumption.    
-    
-  - inversion h3; subst. inversion h4; subst.
-    specialize (IHs0 istate s' h1 h2 H2 H6).
-    inversion IHs0.
-    + inversion H. rewrite e1 in H0; inversion H0.
-    + rewrite e1 in H; inversion H.
-  - (* Cifthen *)
-    inversion h3; subst.
+    specialize (equal_wd_expr_expr2_L _ _ _ h3 H6); intros hz1.
+    specialize (well_formed_expr _ _ _ _ h2 hz1 H4); intros hz2.
+    rm_exists.
+    specialize (f_eval_expr_complete _ _ _ H0); intros hz3.
+    unfold_f_eval_stmt.
+    destruct k.
+    + right; auto.
+    + left. rewrite hz3.
+       destruct x.
+       * specialize (valid_update _ _ _ _ _ v h2 h1); intros hz4.
+         rm_exists.
+         rewrite H.
+         exists x; auto.
+       * specialize (exceptionVal_has_no_typ _ _ _ _ h2 H0 H4); intros hz5.
+         intuition.
+  - (* 2. Sifthen *)
+    inversion h1; subst.
     inversion h4; subst.
-    specialize (IHs0 istate' s' h1 h2 H4 H7). assumption.
-  - left. exists s; auto.  
-  - inversion h3; subst.
+    unfold_f_eval_stmt.
+    destruct k.
+    + right; auto.
+    + fold f_eval_stmt.
+       specialize (IHc _ _ _ k H4 h2 h3 H7).
+       specialize (equal_wd_expr_expr2_L _ _ _ h3 H6); intros hz1.
+       specialize (well_formed_expr _ _ _ _ h2 hz1 H2); intros hz2.
+       rm_exists.
+       specialize (f_eval_expr_complete _ _ _ H0); intros hz3.
+       rewrite hz3.
+       destruct x.
+       * destruct v.
+         rm_contradict.
+         destruct b.
+           assumption.
+           left; exists s; auto.
+       * rm_contradict.
+  - (* 3. Swhile *)
+    inversion h1; subst.
     inversion h4; subst.
-    (**)specialize (equal_wd_expr_expr2_L s istate' b h2 H6). intros h6.
-    (**)specialize (well_formed_expr tb s b Tbool H2 h6 h1). intros h7.
-    inversion h7.
-    + inversion H.
-       specialize (type_consistent s tb b x h1 H2). intros h8.
-       intuition.
-    + inversion H.
-       apply f_eval_expr_complete in H0. 
-       rewrite H0 in y.
-       destruct x in y; intuition.
-  - (* Swhile *)
-    inversion h3; subst.
+    unfold_f_eval_stmt.
+    destruct k.
+    + right; auto.
+    + fold f_eval_stmt.
+       specialize (IHc _ _ _ k H4 h2 h3 H7).
+       specialize (equal_wd_expr_expr2_L _ _ _ h3 H6); intros hz1.
+       specialize (well_formed_expr _ _ _ _ h2 hz1 H2); intros hz2.
+       rm_exists.
+       specialize (f_eval_expr_complete _ _ _ H0); intros hz3.
+       rewrite hz3.
+       destruct x.
+       * destruct v.
+         rm_contradict.
+         destruct b.
+           inversion IHc.
+           rm_exists.
+           rewrite H3.
+             admit. (******** ?????????? ********)
+           rewrite H.
+           right; auto.
+           left; exists s; auto.
+       * rm_contradict.
+  - (* 4. Sseq *)
+    inversion h1; subst.
     inversion h4; subst.
-    specialize (IHs0 istate' s' h1 h2 H4 H7).
-    (**)specialize (symbol_consistent_reserve s tb k' c0 s1 h1 e2). intros h8.
-    specialize (imap_exists s1). intros h9. inversion h9; clear h9.
-    
-    assert(well_defined_stmt2 x (Swhile ast_id b c0) x).
-    (**)specialize (initializationMap_Expr s istate' b k' c0 s1 x   h2 H6 e2 H). intros h9.
-    assert(exists y, well_defined_stmt2 x c0 y).
-    (**)specialize (initializationMap_Stmt s istate' k' c0 s1 s' x h2 e2 H7 H). intros h10.
-    inversion h10; clear h10.
-    exists x0; assumption.
-    inversion H0.
-    apply WD_Swhile2 with (s' := x0); assumption.
-    
-    specialize (IHs1 x x h8 H h3 H0).
-    assumption.
-  - inversion h3; subst.
-    inversion h4; subst.
-    specialize (IHs0 istate' s' h1 h2 H4 H7). 
-    inversion IHs0.
-    + inversion H. rewrite e2 in H0; inversion H0.
-    + rewrite e2 in H; inversion H.
-  - left. exists s; auto.
-  -  inversion h3; subst.
-    inversion h4; subst.
-    (**)specialize (equal_wd_expr_expr2_L s istate' b h2 H6). intros h6.
-    (**)specialize (well_formed_expr tb s b Tbool H2 h6 h1). intros h7.
-    inversion h7.
-    + inversion H.
-       specialize (type_consistent s tb b x h1 H2). intros h8.
-       intuition.
-    + inversion H.
-       apply f_eval_expr_complete in H0. 
-       rewrite H0 in y.
-       destruct x in y; intuition.
+    unfold_f_eval_stmt.
+    destruct k.
+    + right; auto.
+    + fold f_eval_stmt.
+    specialize (IHc1 _ _ _ k H2 h2 h3 H6).
+    inversion IHc1.
+      * rm_exists.
+        rewrite H0.
+        remember H0 as H'0. clear HeqH'0.
+        apply f_eval_stmt_complete in H0.
+        specialize (symbol_consistent_reserve _ _ _ _ h2 H2 H0); intros hz1.
+        specialize (imap_exists x); intros hz2; rm_exists.
+        specialize (f_eval_stmt_complete _ _ _ _ H'0); intros hz2.
+        specialize (initializationMap_consistent _ _ _ _ _ _ _ _ h3 hz2 H6 H7 H); intros hz3.
+        rm_exists.
+        specialize (IHc2 _ _ _ k H4 hz1 H H1).
+        assumption.
+     * rewrite H.
+       right; auto.
+Qed.
 
 
 
